add proof of functional correctness for exp

specs/experimental/rsapss/Spec.RSA.Bignum.fst
@@ -44,20 +44,11 @@ val mont_reduction_f:
 let mont_reduction_f #nBits #cBits rBits nInv_u64 n c i res =
   let res_i = bn_get_bits res (i * 64) ((i + 1)*64) in
   let qi = bn_get_bits (bn_mul nInv_u64 res_i) 0 64 in
-  assert (bn_v qi <= pow2 64 - 1);
   let (c1, res1) = bn_lshift_mul_add n (64*i) qi res in
-  assert (bn_v res1 + uint_v c1 * pow2 (nBits + 1 + rBits) == bn_v res + bn_v n * pow2 (64*i) * bn_v qi); //from bn_lshift_mul_add
-  assert (bn_v res + bn_v n * pow2 (64*i) * bn_v qi <= bn_v c + (pow2 (64*i)-1) * bn_v n + bn_v n * pow2 (64*i) * bn_v qi); //from ind hypo
-  assert (bn_v res + bn_v n * pow2 (64*i) * bn_v qi <= bn_v c + (pow2 (64*i)-1) * bn_v n + bn_v n * pow2 (64*i) * (pow2 64 - 1));
-  assert (bn_v res + bn_v n * pow2 (64*i) * bn_v qi <= bn_v c + pow2 (64*i) * bn_v n - bn_v n + bn_v n * pow2 (64*i) * (pow2 64 - 1));
-  assert (bn_v res + bn_v n * pow2 (64*i) * bn_v qi <= bn_v c + pow2 (64*i) * bn_v n - bn_v n + bn_v n * pow2 (64*i) * pow2 64 - bn_v n * pow2 (64*i));
-  assert (bn_v res + bn_v n * pow2 (64*i) * bn_v qi <= bn_v c - bn_v n + bn_v n * pow2 (64*i) * pow2 64);
-  assert (bn_v res + bn_v n * pow2 (64*i) * bn_v qi <= bn_v c + (pow2 (64*i) * pow2 64 - 1) * bn_v n);
-  pow2_plus (64*i) 64;
-  assert (64*(i+1) <= rBits);
-  assert (bn_v res + bn_v n * pow2 (64*i) * bn_v qi <= bn_v c + (pow2 (64*(i+1)) - 1) * bn_v n);
+  lemma_mont_reduction_fi #nBits #cBits rBits qi n c i res;
   lemma_mont_reduction_f #nBits #cBits rBits n c i;
   assert (bn_v res + bn_v n * pow2 (64*i) * bn_v qi < pow2 (nBits+rBits+1));
+  assert (bn_v res1 + uint_v c1 * pow2 (nBits + 1 + rBits) == bn_v res + bn_v n * pow2 (64*i) * bn_v qi); //from bn_lshift_mul_add
   assert (bn_v res1 == bn_v res + pow2 (64*i) * bn_v qi * bn_v n);
   lemma_mod_plus (bn_v res) (pow2 (64*i) * bn_v qi) (bn_v n); // res1 % n == res % n
   res1
@@ -145,32 +136,26 @@ let from_mont nBits rBits nInv_u64 n a_r =
   small_modulo_lemma_1 (bn_v res) (bn_v n);
   res
 
-val mod_exp_pred:
-  nBits:size_pos ->
-  rBits:size_pos{nBits + 1 < rBits /\ nBits + rBits + 1 < max_size_t /\ rBits % 64 == 0} ->
-  nInv_u64:bignum 64 -> n:bignum nBits{bn_v n > 0} ->
-  bBits:size_pos -> b:bignum bBits ->
-  a0:bignum (nBits+1) -> acc0:bignum (nBits+1) ->
-  i:size_nat{i <= bBits} ->
-  a_acc:tuple2 (bignum (nBits+1)) (bignum (nBits+1)) -> Tot Type0
-let mod_exp_pred nBits rBits nInv_u64 n bBits b a0 acc0 i (a, acc) =
-  if i = 0 then
-    bn_v acc % bn_v n = bn_v acc0 % bn_v n
-  else
-    bn_v acc % bn_v n = ((pow (bn_v a0) (bn_v (bn_get_bits_first b i)) * bn_v acc0) / pow (pow2 rBits) (bn_v (bn_get_bits_first b i))) % bn_v n
-
 val mod_exp_f:
   nBits:size_pos ->
   rBits:size_pos{nBits + 2 < rBits /\ nBits + rBits + 1 < max_size_t /\ rBits % 64 == 0} ->
   nInv_u64:bignum 64 -> n:bignum nBits{bn_v n > 0} ->
   bBits:size_pos -> b:bignum bBits ->
   a0:bignum (nBits+1) -> acc0:bignum (nBits+1) -> Tot (repeatable #(tuple2 (bignum (nBits+1)) (bignum (nBits+1))) #bBits (mod_exp_pred nBits rBits nInv_u64 n bBits b a0 acc0))
-  #reset-options "--z3rlimit 50 --max_fuel 0"
+  #reset-options "--z3rlimit 150 --max_fuel 0"
 let mod_exp_f nBits rBits nInv_u64 n bBits b a0 acc0 i (a, acc) =
-  let acc = if (bn_get_bit b i = 1) then mul_mod_mont nBits rBits nInv_u64 n a acc else acc in
-  let a = mul_mod_mont nBits rBits nInv_u64 n a a in
-  assume (mod_exp_pred nBits rBits nInv_u64 n bBits b a0 acc0 (i+1) (a, acc));
-  (a, acc)
+  let a1 = mul_mod_mont nBits rBits nInv_u64 n a a in
+  assert (bn_v a1 % bn_v n == ((bn_v a * bn_v a) / pow2 rBits) % bn_v n);
+  lemma_mod_exp_a2 nBits rBits nInv_u64 n bBits b a0 acc0 a acc a1 i;
+  assert (bn_v a1 % bn_v n = (pow (bn_v a0) (pow2 (i+1)) / pow (pow2 rBits) (pow2 (i+1) - 1)) % bn_v n);
+  if (bn_get_bit b i = 1) then begin
+    let acc1 = mul_mod_mont nBits rBits nInv_u64 n a acc in
+    lemma_mod_exp_f2 nBits rBits nInv_u64 n bBits b a0 acc0 a acc a1 acc1 i;
+    (a1, acc1) end
+  else begin
+    let acc1 = acc in
+    lemma_mod_exp_f1 nBits rBits nInv_u64 n bBits b a0 acc0 a acc a1 i;
+    (a1, acc1) end
 
 val mod_exp_:
   nBits:size_pos ->
@@ -179,13 +164,15 @@ val mod_exp_:
   a0:bignum (nBits+1) ->
   bBits:size_pos -> b:bignum bBits ->
   acc0:bignum (nBits+1) -> Tot (res:bignum (nBits+1){bn_v res % bn_v n == ((pow (bn_v a0) (bn_v b)) * (bn_v acc0) / pow (pow2 rBits) (bn_v b)) % bn_v n})
-  #reset-options "--z3rlimit 50 --max_fuel 0"
+  #reset-options "--z3rlimit 150 --max_fuel 0"
 let mod_exp_ nBits rBits nInv_u64 n a0 bBits b acc0 =
   let (a, acc) = repeati_inductive bBits
     (mod_exp_pred nBits rBits nInv_u64 n bBits b a0 acc0)
     (fun i (a, acc) -> mod_exp_f nBits rBits nInv_u64 n bBits b a0 acc0 i (a, acc))
     (a0, acc0) in
   assert (bn_v acc % bn_v n = ((pow (bn_v a0) (bn_v (bn_get_bits_first b bBits)) * bn_v acc0) / pow (pow2 rBits) (bn_v (bn_get_bits_first b bBits))) % bn_v n);
+  assert (bn_v b < pow2 bBits);
+  small_modulo_lemma_1 (bn_v b) (pow2 bBits);
   assert (bn_v (bn_get_bits_first b bBits) == bn_v b);
   acc
 
@@ -201,23 +188,24 @@ let mod_exp #aBits nBits n a bBits b =
   let n0 = bn_get_bits n 0 64 in
   let nInv_u64 = bn_from_u64 (mod_inv_u64 (bn_to_u64 n0)) in
   let a_r = to_mont nBits rBits nInv_u64 n r2 a in
-  assert (bn_v a_r % bn_v n == (bn_v a * pow2 rBits) % bn_v n);
   let acc_r = to_mont nBits rBits nInv_u64 n r2 (bn_const_1 #nBits) in
-  assert (bn_v acc_r % bn_v n == pow2 rBits % bn_v n);
   let res_r = mod_exp_ nBits rBits nInv_u64 n a_r bBits b acc_r in
-  assert (bn_v res_r % bn_v n == ((pow (bn_v a_r) (bn_v b)) * (bn_v acc_r) / pow (pow2 rBits) (bn_v b)) % bn_v n);
-  admit();
+  lemma_mod_exp_2 (bn_v n) (bn_v a) (bn_v a_r) (bn_v b) (bn_v acc_r) (pow2 rBits) (bn_v res_r);
   let res = from_mont nBits rBits nInv_u64 n res_r in
+  lemma_mod_mult_div_1 (bn_v res_r) (pow2 rBits) (bn_v n);
+  lemma_mod_mult_div_1 ((pow (bn_v a) (bn_v b)) * pow2 rBits) (pow2 rBits) (bn_v n);
+  multiple_division_lemma (pow (bn_v a) (bn_v b)) (pow2 rBits);
   res
 
 val rsa_blinding:
   #mBits:size_pos ->
   nBits:size_pos{64 <= nBits /\ 2 * 64 * (blocks nBits 64 + 1) < max_size_t} -> n:bignum nBits{0 < bn_v n} ->
-  pBits:size_pos -> p:bignum pBits{0 < bn_v p} ->
-  qBits:size_pos{pBits + qBits + 64 < max_size_t} -> q:bignum qBits{0 < bn_v q /\ bn_v n == bn_v p * bn_v q} ->
-  m:bignum mBits{mBits <= nBits} ->
-  dBits:size_pos{dBits < pBits + qBits + 64} -> d:bignum dBits ->
+  pBits:size_pos -> p:bignum pBits{0 < bn_v p /\ bn_v p < bn_v n} ->
+  qBits:size_pos{pBits + qBits + 64 < max_size_t} -> q:bignum qBits{0 < bn_v q /\ bn_v q < bn_v n /\ bn_v n == bn_v p * bn_v q} ->
+  m:bignum mBits{mBits <= nBits /\ bn_v m < bn_v n} ->
+  dBits:size_pos{dBits < pBits + qBits + 64} -> d:bignum dBits{0 < bn_v d /\ bn_v d < bn_v n} ->
   rBlind:bignum 64 -> Tot (s:bignum nBits{bn_v s == (pow (bn_v m) (bn_v d)) % bn_v n})
+  #reset-options "--z3rlimit 300 --max_fuel 0"
 let rsa_blinding #mBits nBits n pBits p qBits q m dBits d rBlind =
   let bn_1 = bn_const_1 #1 in
   let p1 = bn_sub p bn_1 in
@@ -229,5 +217,6 @@ let rsa_blinding #mBits nBits n pBits p qBits q m dBits d rBlind =
   assume (bn_v d1 + bn_v d < pow2 (pBits + qBits + 64));
   assert (uint_v c == 0);
   let s = mod_exp nBits n m (pBits + qBits + 64) d2 in
+  //lemma_exp_blinding (bn_v n) (bn_v phi_n) (bn_v p) (bn_v q) (bn_v d) (bn_v m) (bn_v rBlind);
   admit();
   s
